\newpage 

\section{Perpendicular Bisector: Reasoning with Algebra}
Prove:  If $C=(x,y)$ is on the perpendicular bisector of the segment from $A=(x_1,y_1)$ and $B=(x_2,y_2)$, then $C$ is equidistant from $A$ and $B$.  

\begin{enumerate}
\item Why is it sufficient to show the following?  
$$(x-x_1)^2+(y-y_1)^2= (x-x_2)^2+(y-y_2)^2$$
\vspace{0.35in}

\item We are given that $C$ is on the perpendicular bisector of $\overline{AB }$.  Explain why we can write:  
$$y-\frac{y_1+y_2}{2} = -\left(\frac{x_2-x_1}{y_2-y_1}\right)\left(x-\frac{x_1+x_2}{2}\right)$$
\vspace{0.5in}
\item In the spaces that follow each equation, provide a supporting explanation for each step.  
\vspace{0.35in}
$$2y-y_1-y_2 = -\left(\frac{x_2-x_1}{y_2-y_1}\right)\left(2x-x_1-x_2\right)$$
\vspace{0.35in}
$$(y-y_1)+(y-y_2) = -\left(\frac{x_2-x_1}{y_2-y_1}\right)\left((x-x_1)+(x-x_2)\right)$$
\vspace{0.35in}
$$(y_2-y_1)\left[(y-y_1)+(y-y_2)\right]= (x_1-x_2)\left[(x-x_1)+(x-x_2)\right]$$
\vspace{0.35in}
$$\left[(y-y_1)-(y-y_2)\right]\left[(y-y_1)+(y-y_2)\right]= \left[(x-x_2)-(x-x_1)\right]\left[(x-x_2)+(x-x_1)\right]$$
\vspace{0.35in}
$$(y-y_1)^2-(y-y_2)^2= (x-x_2)^2-(x-x_1)^2$$
\vspace{0.35in}
$$(x-x_1)^2+(y-y_1)^2= (x-x_2)^2+(y-y_2)^2$$
\vspace{0.35in}
\item How does this algebraic argument prove the statement generally, for any points $A$, $B$, and $C$?  
\end{enumerate}
